See [[The Integral]], [[The Differential]].
$$
\begin{aligned}
\nabla\cdot\mathbf{E} &= \frac{\rho}{\varepsilon_0} &&\text{(Gauss's law)}\\[6pt]
\nabla\cdot\mathbf{B} &= 0 &&\text{(Gauss's law for magnetism)}\\[6pt]
\nabla\times\mathbf{E} &= -\frac{\partial \mathbf{B}}{\partial t} &&\text{(Faraday's law)}\\[6pt]
\nabla\times\mathbf{B} &= \mu_0\mathbf{J} + \mu_0\varepsilon_0\frac{\partial \mathbf{E}}{\partial t} &&\text{(Ampère–Maxwell law)}
\end{aligned}
$$

$$
\begin{aligned}
\oint_{\partial V}\mathbf{E}\cdot d\mathbf{A} &= \frac{1}{\varepsilon_0}\int_V \rho\,dV \\[6pt]
\oint_{\partial V}\mathbf{B}\cdot d\mathbf{A} &= 0 \\[6pt]
\oint_{\partial S}\mathbf{E}\cdot d\boldsymbol{\ell} &= -\frac{d}{dt}\iint_S \mathbf{B}\cdot d\mathbf{A} \\[6pt]
\oint_{\partial S}\mathbf{B}\cdot d\boldsymbol{\ell} &= \mu_0\iint_S \mathbf{J}\cdot d\mathbf{A} + \mu_0\varepsilon_0\frac{d}{dt}\iint_S \mathbf{E}\cdot d\mathbf{A}
\end{aligned}
$$

$$
\begin{aligned}
\nabla\cdot\mathbf{D} &= \rho_{\mathrm{free}} \\[6pt]
\nabla\cdot\mathbf{B} &= 0 \\[6pt]
\nabla\times\mathbf{E} &= -\frac{\partial \mathbf{B}}{\partial t} \\[6pt]
\nabla\times\mathbf{H} &= \mathbf{J}_{\mathrm{free}} + \frac{\partial \mathbf{D}}{\partial t}
\end{aligned}
$$

$$
\nabla\cdot\mathbf{J} + \frac{\partial \rho}{\partial t} = 0
$$


